module plfa.part1.Decidable where

import Relation.Binary.PropositionalEquality as Eq
open Eq using (_≡_; refl)
open Eq.≡-Reasoning
open import Data.Nat using (ℕ; zero; suc)
open import Data.Product using (_×_) renaming (_,_ to ⟨_,_⟩)
open import Data.Sum using (_⊎_; inj₁; inj₂)
open import Relation.Nullary using (¬_)
open import Relation.Nullary.Negation using () renaming (contradiction to ¬¬-intro)
open import Data.Unit using (⊤; tt)
open import Data.Empty using (⊥; ⊥-elim)
open import plfa.part1.Relations using (_<_; z<s; s<s)
open import plfa.part1.Isomorphism using (_⇔_)

-- Evidence vs computation

infix 4 _≤_

data _≤_ : ℕ → ℕ → Set where
  z≤n : ∀ {n : ℕ} → zero ≤ n
  s≤s : ∀ {m n : ℕ} → m ≤ n → suc m ≤ suc n

_ : 2 ≤ 4
_ = s≤s (s≤s z≤n)

¬4≤2 : ¬ (4 ≤ 2)
¬4≤2 (s≤s (s≤s ()))

data Bool : Set where
  true  : Bool
  false : Bool

infix 4 _≤ᵇ_

_≤ᵇ_ : ℕ → ℕ → Bool
zero ≤ᵇ n = true
suc m ≤ᵇ zero = false
suc m ≤ᵇ suc n = m ≤ᵇ n

_ : (2 ≤ᵇ 4) ≡ true
_ = begin
  2 ≤ᵇ 4 ≡⟨⟩
  1 ≤ᵇ 3 ≡⟨⟩
  0 ≤ᵇ 2 ≡⟨⟩
  true   ∎

_ : (4 ≤ᵇ 2) ≡ false
_ = begin
  4 ≤ᵇ 2 ≡⟨⟩
  3 ≤ᵇ 1 ≡⟨⟩
  2 ≤ᵇ 0 ≡⟨⟩
  false  ∎

-- Relating evidence and computation

T : Bool → Set
T true  = ⊤
T false = ⊥

T→≡ : ∀ (b : Bool) → T b → b ≡ true
T→≡ true  tt = refl
T→≡ false ()

≡→T : ∀ {b : Bool} → b ≡ true → T b
≡→T refl = tt

≤ᵇ→≤ : ∀ (m n : ℕ) → T (m ≤ᵇ n) → m ≤ n
≤ᵇ→≤ zero n tt = z≤n
≤ᵇ→≤ (suc m) (suc n) t = s≤s (≤ᵇ→≤ m n t)

≤→≤ᵇ : ∀ {m n : ℕ} → m ≤ n → T (m ≤ᵇ n)
≤→≤ᵇ z≤n       = tt
≤→≤ᵇ (s≤s m≤n) = ≤→≤ᵇ m≤n

-- The best of both worlds

data Dec (A : Set): Set where
  yes :   A → Dec A
  no  : ¬ A → Dec A

¬s≤z : ∀ {m : ℕ} → ¬ (suc m ≤ zero)
¬s≤z ()

¬s≤s : ∀ {m n : ℕ} → ¬ (m ≤ n) → ¬ (suc m ≤ suc n)
¬s≤s ¬m≤n (s≤s m≤n) = ¬m≤n m≤n

_≤?_ : ∀ (m n : ℕ) → Dec (m ≤ n)
zero ≤? n = yes z≤n
suc m ≤? zero = no ¬s≤z
suc m ≤? suc n with m ≤? n
...               | yes m≤n = yes (s≤s m≤n)
...               | no ¬m≤n = no (¬s≤s ¬m≤n)

-- Exercise: _<?_

¬z<z : ¬ (zero < zero)
¬z<z ()

¬s<z : ∀ {n : ℕ} → ¬ (suc n < zero)
¬s<z ()

¬s<s : ∀ {m n : ℕ} → ¬ (m < n) → ¬ (suc m < suc n)
¬s<s ¬m<n (s<s m<n) = ¬m<n m<n

_<?_ : ∀ (m n : ℕ) → Dec (m < n)
zero <? zero = no ¬z<z
zero <? suc n = yes z<s
suc m <? zero = no ¬s<z
suc m <? suc n with m <? n
...               | yes m<n = yes (s<s m<n)
...               | no ¬m<n = no (¬s<s ¬m<n)

-- Exercise: _≡ℕ?_

¬s≡z : ∀ {m : ℕ} → ¬ (zero ≡ suc m)
¬s≡z ()

¬z≡s : ∀ {m : ℕ} → ¬ (suc m ≡ zero)
¬z≡s ()

¬s≡s : ∀ {m n : ℕ} → ¬ (m ≡ n) → ¬ (suc m ≡ suc n)
¬s≡s ¬m≡n refl = ¬m≡n refl

_≡ℕ?_ : ∀ (m n : ℕ) → Dec (m ≡ n)
zero ≡ℕ? zero = yes refl
zero ≡ℕ? suc n = no ¬s≡z
suc m ≡ℕ? zero = no ¬z≡s
suc m ≡ℕ? suc n with m ≡ℕ? n
...                | yes m≡n = yes (Eq.cong suc m≡n)
...                | no ¬m≡n = no (¬s≡s ¬m≡n)
